Substitution composition

theories/Example/Substitution.v
@@ -3,31 +3,19 @@ From Nominal Require Import Lambda.
 Section Subs.
     Context (a: Name) (N: Λ).
 
-    Instance: Proper (eq ==> equiv) (Var).
-    Proof. repeat intro; rewrite H; reflexivity. Qed.
-
-    Instance: Proper (equiv ==> equiv ==> equiv) (App).
-    Proof. repeat intro; apply AeqAppC; auto. Qed.
-
-    Definition S: NameSet := support a ∪ support N.
-
     Definition fvar: Name →ₛ Λ.
-       refine (λₛ⟦S⟧ b, if decide (a = b) then N else Var b).
+       refine (λₛ⟦support a ∪ support N⟧ b, if decide (a = b) then N else Var b).
     Proof.
-       intros c d ? ? w. destruct (decide (a = w)); subst.
-          - rewrite name_action_neither.
-            + destruct (decide _); try congruence; rewrite support_spec; set_solver.
-            + set_solver.
-            + set_solver.
+       intros c d ? ? w; destruct (decide (a = w)); subst.
+          - rewrite name_action_neither; [| set_solver | set_solver].
+            destruct (decide _); try congruence; rewrite support_spec; set_solver.
           - destruct (decide (c = w)), (decide (d = w)); subst.
             + rewrite !perm_action_equal; unfold action,name_action; rewrite perm_swap_left.
               destruct (decide _); try congruence; reflexivity.
-            + rewrite perm_swap_left; destruct (decide _); subst; try congruence.
-               * set_solver.
-               * rewrite term_perm_var, perm_swap_right; reflexivity.
-            + rewrite perm_swap_right; destruct (decide _); subst; try congruence.
-               * set_solver.
-               * rewrite term_perm_var, perm_swap_left; reflexivity.
+            + rewrite perm_swap_left; destruct (decide _); subst; try congruence; [set_solver |].
+              rewrite term_perm_var, perm_swap_right; reflexivity.
+            + rewrite perm_swap_right; destruct (decide _); subst; try congruence; [set_solver |].
+              rewrite term_perm_var, perm_swap_left; reflexivity.
             + rewrite perm_swap_neither; try destruct (decide _); subst; try congruence.
               rewrite term_perm_var,perm_swap_neither; set_solver.
     Defined.
@@ -44,30 +32,20 @@ Section Subs.
     Proof.
        - intros [b x] [c y] [H1 H2]; simpl in *; apply AeqAbsC with (L := ∅); intros d ?; rewrite H1; 
          apply term_perm_alpha; assumption.
-       - intros w z ? ? [b x]; simpl in *; rewrite term_perm_abs, !perm_action_duplicate; apply AeqAbsC with (L := ∅).
-         intros ? ?; rewrite !perm_action_duplicate; reflexivity.
+       - intros w z ? ? [b x]; simpl in *; rewrite term_perm_abs, !perm_action_duplicate; reflexivity.
     Defined.
 
-    Fact fvarL: f_supp fvar ⊆ S. Proof. set_solver. Qed.
-    Fact fappL: f_supp fapp ⊆ S. Proof. set_solver. Qed.
-    Fact flamL: f_supp flam ⊆ S. Proof. set_solver. Qed.
-
-    Fact fcb: ∃ a, a # flam ∧ ∀ x, a # flam (a,x).
+    Fact flam_fcb: ∃ a, a # flam ∧ ∀ x, a # flam (a,x).
     Proof.
-       destruct (exist_fresh (support flam ∪ support a ∪ support N)) as [w Hw].
-       exists w; split.
+       destruct (exist_fresh (support flam ∪ support a ∪ support N)) as [w Hw]; exists w; split.
        - apply support_fresh; set_solver.
-       - intros x. destruct (exist_fresh (support flam ∪ support a ∪ support N ∪ support x ∪ support w ∪ support (flam (w, x)) ∪ fv (Lam w x))) as [z Hz].
-         exists z; split.
-         + set_solver.
-         + rewrite fun_equivar, support_spec.
-           * rewrite prod_act, perm_swap_left; simpl; symmetry; apply aeq_lam_swap_notin; set_solver.
-           * set_solver.
-           * set_solver.
-    Qed.
+       - intros x; destruct (exist_fresh (support flam ∪ support a ∪ support N ∪ support x ∪ support w ∪ support (flam (w, x)) ∪ fv (Lam w x))) as [z Hz].
+         exists z; split; [set_solver |].
+         rewrite fun_equivar, support_spec; [| set_solver | set_solver].
+         rewrite prod_act, perm_swap_left; simpl; symmetry; apply aeq_lam_swap_notin; set_solver.
+   Qed.
 
-    Definition subst := alpha_rec (support a ∪ support N) fvar fapp flam fvarL fappL flamL fcb.
-
+    Definition subst := alpha_rec (support a ∪ support N) fvar fapp flam ltac:(set_solver) ltac:(set_solver) ltac:(set_solver) flam_fcb.
 End Subs.
 
 Notation " '[' a ':=' N ']' M " := (subst a N M) (at level 59, M at next level, format "[ a  :=  N ] M").
@@ -81,5 +59,41 @@ Proof. unfold subst; rewrite alpha_rec_app; unfold fapp; simpl; reflexivity. Qed
 Lemma subst_lam (a b: Name) (m n: Λ): a ≠ b → a ∉ support n → [b := n](Lam a m) ≡ Lam a ([b := n]m).
 Proof. 
  intros; assert (HH: Lam a ([b := n]m) ≡ flam(a, ([b := n]m))). { simpl; reflexivity. }
- rewrite HH; clear HH; unfold subst; apply alpha_rec_lam; apply not_elem_of_union; split; set_solver.
+ rewrite HH; clear HH; unfold subst; apply alpha_rec_lam. apply not_elem_of_union; split; set_solver.
+Qed.
+
+Opaque subst.
+
+Lemma subst_aeq (a: Name) (m p q: Λ): p ≡ q → [a := p]m ≡ [a := q]m.
+Proof.
+   intros; generalize dependent m; set (P := fun t => [a := p]t ≡ [a := q]t).
+   apply (alpha_ind (support a ∪ support p ∪ support q) P); subst P; intros; simpl in *.
+   - unfold αCompat; intros; rewrite <-H0; auto.
+   - rewrite !subst_var; destruct (decide _); auto.
+   - rewrite !subst_app; rewrite H0,H1; reflexivity.
+   - rewrite !subst_lam; [rewrite H1 | | | |]; set_solver.
+Qed.
+
+Lemma subst_neq_var (a: Name) (m n: Λ): a # m → [a := n]m ≡ m.
+Proof.
+   generalize dependent m; set (P := fun t => a # t → [a := n]t ≡ t). apply (alpha_ind (support a ∪ support n) P); subst P; simpl in *.
+   - repeat intro; rewrite <-H; apply H0; rewrite H; auto. 
+   - intros b H; rewrite subst_var; apply var_fresh in H; destruct (decide _); subst; try congruence; reflexivity.
+   - simpl in *; intros p q ? ? ?; apply app_fresh in H1 as []; rewrite subst_app; rewrite H,H0; auto.
+   - simpl in *; intros b m ? ? ?; rewrite subst_lam; [| set_solver | set_solver].
+     rewrite H0; [reflexivity | apply lam_fresh in H1 as []; subst; set_solver].
+Qed.
+
+Lemma subst_comp (a b: Name) (m p q: Λ): 
+   a ≠ b → a ∉ fv p → [b := p]([a := q]m) ≡ [a := ([b := p]q)]([b := p]m).
+Proof.
+   intros; generalize dependent m; set (P := fun t => [b := p]([a := q]t) ≡ [a := [b := p]q]([b := p]t)).
+   apply (alpha_ind (support a ∪ support b ∪ support p ∪ support q ∪ support ([b := p]q)) P); subst P; simpl in *.
+   - unfold αCompat; intros; rewrite <-H1; assumption.
+   - intros c; destruct (decide (a = c)), (decide (b = c)); subst; try congruence;
+      repeat (rewrite !subst_var; repeat destruct (decide _); subst; try congruence); auto.
+      rewrite subst_neq_var; [| apply support_fresh]; auto.
+   - intros; rewrite !subst_app; constructor; auto.
+   - intros c ? ? ?; rewrite !subst_lam.
+     1:(rewrite H2; reflexivity). all:set_solver.
 Qed.
